<?xml version="1.0"?>


<!DOCTYPE rdf:RDF [
    <!ENTITY dct "http://purl.org/dc/terms/" >
    <!ENTITY atpir-fi "http://purl.org/NET/atpir-cw" >
    <!ENTITY owl "http://www.w3.org/2002/07/owl#" >
    <!ENTITY xsd "http://www.w3.org/2001/XMLSchema#" >
    <!ENTITY xml "http://www.w3.org/XML/1998/namespace" >
    <!ENTITY rdfs "http://www.w3.org/2000/01/rdf-schema#" >
    <!ENTITY rdf "http://www.w3.org/1999/02/22-rdf-syntax-ns#" >
]>


<rdf:RDF xmlns="&atpir-fi;#"
     xml:base="http://purl.org/NET/atpir-cw"
     xmlns:dct="http://purl.org/dc/terms/"
     xmlns:rdf="http://www.w3.org/1999/02/22-rdf-syntax-ns#"
     xmlns:atpir-fi="http://purl.org/NET/atpir-cw"
     xmlns:owl="http://www.w3.org/2002/07/owl#"
     xmlns:xml="http://www.w3.org/XML/1998/namespace"
     xmlns:xsd="http://www.w3.org/2001/XMLSchema#"
     xmlns:rdfs="http://www.w3.org/2000/01/rdf-schema#">
    <owl:Ontology rdf:about="http://purl.org/NET/atpir-cw">
        <rdfs:label>Complaint Workflow Ontology</rdfs:label>
        <dct:contributor>Victor Rodriguez-Doncel</dct:contributor>
        <dct:contributor>Cristiana Santos</dct:contributor>
        <owl:versionInfo>1.0</owl:versionInfo>
        <rdfs:comment>This is an ontology on the workflow on complaints on Flight Incidents.
The ontology defines the integrative workflow upon which a consumer might bring a complaint in a valid and complete way when a dispute arises against an airline
</rdfs:comment>
        <dct:license rdf:resource="http://purl.org/NET/rdflicense/cc-by"/>
    </owl:Ontology>
    


    <!-- 
    ///////////////////////////////////////////////////////////////////////////////////////
    //
    // Annotation properties
    //
    ///////////////////////////////////////////////////////////////////////////////////////
     -->

    


    <!-- http://purl.org/NET/atpir-cw#hasAirline -->

    <owl:AnnotationProperty rdf:about="&atpir-fi;#hasAirline">
        <rdfs:domain rdf:resource="&atpir-fi;Flight"/>
    </owl:AnnotationProperty>
    


    <!-- 
    ///////////////////////////////////////////////////////////////////////////////////////
    //
    // Object Properties
    //
    ///////////////////////////////////////////////////////////////////////////////////////
     -->

    


    <!-- http://purl.org/NET/atpir-cw#hasActionStep -->

    <owl:ObjectProperty rdf:about="&atpir-fi;#hasActionStep">
        <rdfs:comment>Declares the step related to a workflow</rdfs:comment>
        <rdfs:range rdf:resource="&atpir-fi;#ActionStep"/>
        <rdfs:domain rdf:resource="&atpir-fi;#ComplaintWorkflow"/>
        <rdfs:subPropertyOf rdf:resource="&owl;topObjectProperty"/>
    </owl:ObjectProperty>
    


    <!-- http://purl.org/NET/atpir-cw#hasAirCarrierDetails -->

    <owl:ObjectProperty rdf:about="&atpir-fi;#hasAirCarrierDetails">
        <rdfs:domain rdf:resource="&atpir-fi;#AirCarrier"/>
    </owl:ObjectProperty>
    


    <!-- http://purl.org/NET/atpir-cw#hasFormat -->

    <owl:ObjectProperty rdf:about="&atpir-fi;#hasFormat">
        <rdfs:domain rdf:resource="&atpir-fi;#ComplainingToTheAirCarrier"/>
        <rdfs:range rdf:resource="&atpir-fi;#OnlineComplaining"/>
    </owl:ObjectProperty>
    


    <!-- http://purl.org/NET/atpir-cw#hasOfflineFormat -->

    <owl:ObjectProperty rdf:about="&atpir-fi;#hasOfflineFormat">
        <rdfs:domain rdf:resource="&atpir-fi;#Complaint"/>
        <rdfs:subPropertyOf rdf:resource="&owl;topObjectProperty"/>
    </owl:ObjectProperty>
    


    <!-- http://purl.org/NET/atpir-cw#hasOnlineFormat -->

    <owl:ObjectProperty rdf:about="&atpir-fi;#hasOnlineFormat">
        <rdfs:domain rdf:resource="&atpir-fi;#Complaint"/>
        <rdfs:subPropertyOf rdf:resource="&owl;topObjectProperty"/>
    </owl:ObjectProperty>
    


    <!-- http://purl.org/NET/atpir-cw#hasParty -->

    <owl:ObjectProperty rdf:about="&atpir-fi;#hasParty">
        <rdfs:comment>Declares a party that is in a complaint</rdfs:comment>
        <rdfs:domain rdf:resource="&atpir-fi;#Complaint"/>
        <rdfs:range rdf:resource="&atpir-fi;#Party"/>
    </owl:ObjectProperty>
    


    <!-- http://purl.org/NET/atpir-cw#hasPassengerDetails -->

    <owl:ObjectProperty rdf:about="&atpir-fi;#hasPassengerDetails">
        <rdfs:domain rdf:resource="&atpir-fi;#Passenger"/>
    </owl:ObjectProperty>
    


    <!-- http://purl.org/NET/atpir-cw#hasPreviousStep -->

    <owl:ObjectProperty rdf:about="&atpir-fi;#hasPreviousStep">
        <rdfs:comment>Declares the order of the action steps of the workflow</rdfs:comment>
        <rdfs:domain rdf:resource="&atpir-fi;#ActionStep"/>
        <rdfs:range rdf:resource="&atpir-fi;#ActionStep"/>
    </owl:ObjectProperty>
    


    <!-- http://purl.org/NET/atpir-cw#hasProofDocuments -->

    <owl:ObjectProperty rdf:about="&atpir-fi;#hasProofDocuments">
        <rdfs:domain rdf:resource="&atpir-fi;#AddingProofDocument"/>
        <rdfs:range rdf:resource="&atpir-fi;#ProofDocument"/>
    </owl:ObjectProperty>
    


    <!-- http://purl.org/NET/atpir-cw#hasWorkflow -->

    <owl:ObjectProperty rdf:about="&atpir-fi;#hasWorkflow">
        <rdfs:domain rdf:resource="&atpir-fi;#Complaint"/>
        <rdfs:range rdf:resource="&atpir-fi;#ComplaintWorkflow"/>
    </owl:ObjectProperty>
    


    <!-- 
    ///////////////////////////////////////////////////////////////////////////////////////
    //
    // Data properties
    //
    ///////////////////////////////////////////////////////////////////////////////////////
     -->

    


    <!-- http://purl.org/NET/atpir-cw#AirCarrierAddress -->

    <owl:DatatypeProperty rdf:about="&atpir-fi;#AirCarrierAddress">
        <rdfs:comment>The address of the air carrier.</rdfs:comment>
        <rdfs:domain rdf:resource="&atpir-fi;#AirCarrier"/>
        <rdfs:range rdf:resource="&xsd;string"/>
    </owl:DatatypeProperty>
    


    <!-- http://purl.org/NET/atpir-cw#AirCarrierName -->

    <owl:DatatypeProperty rdf:about="&atpir-fi;#AirCarrierName">
        <rdfs:comment>The identification of the air carrier.</rdfs:comment>
        <rdfs:domain rdf:resource="&atpir-fi;#AirCarrier"/>
        <rdfs:range rdf:resource="&xsd;string"/>
    </owl:DatatypeProperty>
    


    <!-- http://purl.org/NET/atpir-cw#BookingReference -->

    <owl:DatatypeProperty rdf:about="&atpir-fi;#BookingReference">
        <rdfs:comment>The booking reference (also called Passenger Name Record or PNR) is an alphanumeric code (sequence comprised of six letters and/or numbers in length) used to uniquely identify one specific booking reservation. It can be found on the receipt the passenger has received after completing the act of booking.</rdfs:comment>
        <rdfs:domain rdf:resource="&atpir-fi;#Passenger"/>
        <rdfs:range rdf:resource="&xsd;string"/>
    </owl:DatatypeProperty>
    


    <!-- http://purl.org/NET/atpir-cw#PassengerChildIdentification -->

    <owl:DatatypeProperty rdf:about="&atpir-fi;#PassengerChildIdentification">
        <rdfs:comment>Identification of the passenger&apos;s child.</rdfs:comment>
        <rdfs:domain rdf:resource="&atpir-fi;#Passenger"/>
        <rdfs:subPropertyOf rdf:resource="&atpir-fi;#PassengerContacts"/>
        <rdfs:range rdf:resource="&xsd;Name"/>
    </owl:DatatypeProperty>
    


    <!-- http://purl.org/NET/atpir-cw#PassengerContacts -->

    <owl:DatatypeProperty rdf:about="&atpir-fi;#PassengerContacts">
        <rdfs:comment>The contacts of the passenger, such as telephone, mobile phone and email address.</rdfs:comment>
        <rdfs:domain rdf:resource="&atpir-fi;#Passenger"/>
        <rdfs:range rdf:resource="&xsd;integer"/>
    </owl:DatatypeProperty>
    


    <!-- http://purl.org/NET/atpir-cw#PassengerCountry -->

    <owl:DatatypeProperty rdf:about="&atpir-fi;#PassengerCountry">
        <rdfs:comment>The country of the passenger.</rdfs:comment>
        <rdfs:domain rdf:resource="&atpir-fi;#Passenger"/>
        <rdfs:range rdf:resource="&xsd;string"/>
    </owl:DatatypeProperty>
    


    <!-- http://purl.org/NET/atpir-cw#PassengerFullAddress -->

    <owl:DatatypeProperty rdf:about="&atpir-fi;#PassengerFullAddress">
        <rdfs:comment>The passenger&apos;s full address.</rdfs:comment>
        <rdfs:domain rdf:resource="&atpir-fi;#Passenger"/>
        <rdfs:range rdf:resource="&xsd;string"/>
    </owl:DatatypeProperty>
    


    <!-- http://purl.org/NET/atpir-cw#PassengerFullName -->

    <owl:DatatypeProperty rdf:about="&atpir-fi;#PassengerFullName">
        <rdfs:comment>The passenger&apos;s full name.</rdfs:comment>
        <rdfs:domain rdf:resource="&atpir-fi;#Passenger"/>
        <rdfs:range rdf:resource="&xsd;Name"/>
    </owl:DatatypeProperty>
    


    <!-- http://purl.org/NET/atpir-cw#TicketNumber -->

    <owl:DatatypeProperty rdf:about="&atpir-fi;#TicketNumber">
        <rdfs:comment>The ticket number is a 13-digit number that uniquely identifies the air carrier ticket that was issued to the passenger.
It includes the air carrier&apos;s 3-digit ticketing code, a 4-digit form number, a 6-digit serial number, and sometimes a check digit. 
The sources to locate the ticket number are boarding pass and the ticket receipt.</rdfs:comment>
        <rdfs:domain rdf:resource="&atpir-fi;#Complaint"/>
        <rdfs:range rdf:resource="&xsd;integer"/>
    </owl:DatatypeProperty>
    


    <!-- 
    ///////////////////////////////////////////////////////////////////////////////////////
    //
    // Classes
    //
    ///////////////////////////////////////////////////////////////////////////////////////
     -->

    


    <!-- http://purl.org/NET/atpir-cw#ActionStep -->

    <owl:Class rdf:about="&atpir-fi;#ActionStep">
        <rdfs:comment>Specific set of steps to lodge a complaint.</rdfs:comment>
    </owl:Class>
    


    <!-- http://purl.org/NET/atpir-cw#AddingProofDocument -->

    <owl:Class rdf:about="&atpir-fi;#AddingProofDocument">
        <rdfs:subClassOf rdf:resource="&atpir-fi;#ActionStep"/>
        <rdfs:comment>Step of the complaint workflow which consists of adding proof documents to the complaint.</rdfs:comment>
    </owl:Class>
    


    <!-- http://purl.org/NET/atpir-cw#AirCarrier -->

    <owl:Class rdf:about="&atpir-fi;#AirCarrier">
        <rdfs:subClassOf rdf:resource="&atpir-fi;#Party"/>
        <rdfs:isDefinedBy>Air carrier means an air transport that provides air transport services for passengers and/or freight.
Airlines lease or own their aircraft, undertaking with a valid operating licence, Article 2 (a), Regulation 261/2004.
</rdfs:isDefinedBy>
    </owl:Class>
    


    <!-- http://purl.org/NET/atpir-cw#BaggageInventoryForm -->

    <owl:Class rdf:about="&atpir-fi;#BaggageInventoryForm">
        <rdfs:subClassOf rdf:resource="&atpir-fi;#ProofDocument"/>
        <rdfs:comment>Template or form that the passenger needs to to fill for reporting the missing baggage with information regarding the color and shape of the baggage and the items contained in the baggage.</rdfs:comment>
    </owl:Class>
    


    <!-- http://purl.org/NET/atpir-cw#BoardingPass -->

    <owl:Class rdf:about="&atpir-fi;#BoardingPass">
        <rdfs:subClassOf rdf:resource="&atpir-fi;#ProofDocument"/>
        <rdfs:comment>Boarding Pass means a valid document, or something equivalent in paperless form, including electronic form, issued or authorised by the air carrier or its authorised agent, giving a passenger permission to board the airplane for a particular flight. As a minimum, it identifies the passenger, the flight number, and the date and scheduled time for departure. In some cases, flyers can check in online and print the boarding passes themselves.</rdfs:comment>
    </owl:Class>
    


    <!-- http://purl.org/NET/atpir-cw#CabinCrew -->

    <owl:Class rdf:about="&atpir-fi;#CabinCrew">
        <rdfs:subClassOf rdf:resource="&atpir-fi;#AirCarrier"/>
        <rdfs:comment>Group of individuals who work in the passenger area, which is also known as the cabin. People who work in the cabin may be referred to as flight attendants, stewards or stewardesses, or air hosts or hostesses.</rdfs:comment>
    </owl:Class>
    


    <!-- http://purl.org/NET/atpir-cw#CallCenter -->

    <owl:Class rdf:about="&atpir-fi;#CallCenter">
        <rdfs:subClassOf rdf:resource="&atpir-fi;#AirCarrier"/>
        <rdfs:comment>Call Center is a centralised office used for the purpose of receiving or transmitting a large volume of requests by telephone. An inbound call centre is operated by a company to administer incoming product support or information inquiries from consumers.</rdfs:comment>
    </owl:Class>
    


    <!-- http://purl.org/NET/atpir-cw#Captain -->

    <owl:Class rdf:about="&atpir-fi;#Captain">
        <rdfs:subClassOf rdf:resource="&atpir-fi;#TechnicalCrew"/>
        <rdfs:comment>Captain is the person aboard the aircraft who is ultimately responsible for its operation and safety during flight, or pilot in command (PIC).</rdfs:comment>
    </owl:Class>
    


    <!-- http://purl.org/NET/atpir-cw#ComplainingToTheAirCarrier -->

    <owl:Class rdf:about="&atpir-fi;#ComplainingToTheAirCarrier">
        <rdfs:subClassOf rdf:resource="&atpir-fi;#ActionStep"/>
        <rdfs:comment>First step of the complaint workflow in order to lodge a complaint to the air carrier.
</rdfs:comment>
    </owl:Class>
    


    <!-- http://purl.org/NET/atpir-cw#Complaint -->

    <owl:Class rdf:about="&atpir-fi;#Complaint">
        <rdfs:comment>Any formal legal document that sets out the facts (cause of action) and legal reasons that the consumer believes are sufficient to support a claim against the company </rdfs:comment>
    </owl:Class>
    


    <!-- http://purl.org/NET/atpir-cw#ComplaintWorkflow -->

    <owl:Class rdf:about="&atpir-fi;#ComplaintWorkflow">
        <rdfs:comment>Life-cycle for handling a complaint which consists in a specific set of steps to lodge a complaint.</rdfs:comment>
    </owl:Class>
    


    <!-- http://purl.org/NET/atpir-cw#CopyRecord -->

    <owl:Class rdf:about="&atpir-fi;#CopyRecord">
        <rdfs:subClassOf rdf:resource="&atpir-fi;#ProofDocument"/>
        <rdfs:comment>Record of the copy of the complaint.</rdfs:comment>
    </owl:Class>
    


    <!-- http://purl.org/NET/atpir-cw#FlightAttendant -->

    <owl:Class rdf:about="&atpir-fi;#FlightAttendant">
        <rdfs:subClassOf rdf:resource="&atpir-fi;#CabinCrew"/>
        <rdfs:comment>Is the crew member responsible for the safety of passengers.</rdfs:comment>
    </owl:Class>
    


    <!-- http://purl.org/NET/atpir-cw#GroundHandling -->

    <owl:Class rdf:about="&atpir-fi;#GroundHandling">
        <rdfs:subClassOf rdf:resource="&atpir-fi;#AirCarrier"/>
        <rdfs:comment>Ground handling addresses the many service requirements of an airliner between the time it arrives at a terminal gate and the time it departs on its next flight.Many airlines subcontract ground handling to airports, handling agents or even to another airline.</rdfs:comment>
    </owl:Class>
    


    <!-- http://purl.org/NET/atpir-cw#Invoice -->

    <owl:Class rdf:about="&atpir-fi;#Invoice">
        <rdfs:subClassOf rdf:resource="&atpir-fi;#ProofDocument"/>
        <rdfs:comment>An invoice, bill or tab is a commercial document issued by a seller to a buyer, relating to any sale transaction and indicating the products, quantities, and agreed prices for products or services the seller has provided the buyer.</rdfs:comment>
    </owl:Class>
    


    <!-- http://purl.org/NET/atpir-cw#NationalEnforcementBody -->

    <owl:Class rdf:about="&atpir-fi;#NationalEnforcementBody">
        <rdfs:subClassOf rdf:resource="&atpir-fi;#AirCarrier"/>
        <rdfs:comment>A body responsible for the enforcement of this Regulation as regards flights from airports situated on its territory and flights from a third country to such airports. Where appropriate, this body shall take the measures necessary to ensure that the rights of passengers are respected. Passengers who believe they have not been treated correctly should contact the body in the country where the incident took place, Article 16of the Regulation (EC) 261/2004.</rdfs:comment>
    </owl:Class>
    


    <!-- http://purl.org/NET/atpir-cw#OfflineComplaining -->

    <owl:Class rdf:about="&atpir-fi;#OfflineComplaining">
        <rdfs:subClassOf rdf:resource="&atpir-fi;#ComplainingToTheAirCarrier"/>
        <rdfs:comment>Offline format of the document that is used to lodge a complaint. </rdfs:comment>
    </owl:Class>
    


    <!-- http://purl.org/NET/atpir-cw#OnlineComplaining -->

    <owl:Class rdf:about="&atpir-fi;#OnlineComplaining">
        <rdfs:subClassOf rdf:resource="&atpir-fi;#ComplainingToTheAirCarrier"/>
        <rdfs:comment>Online format of the document that is used to lodge a complaint. </rdfs:comment>
    </owl:Class>
    


    <!-- http://purl.org/NET/atpir-cw#Party -->

    <owl:Class rdf:about="&atpir-fi;#Party">
        <rdfs:comment>Agents that might be involved in a process.</rdfs:comment>
    </owl:Class>
    


    <!-- http://purl.org/NET/atpir-cw#Passenger -->

    <owl:Class rdf:about="&atpir-fi;#Passenger">
        <rdfs:subClassOf rdf:resource="&atpir-fi;#Party"/>
        <rdfs:comment>A passenger is a natural person independent of age who intends to conclude, or has consented to, a contract of air carriage with the provider of a transport service.</rdfs:comment>
    </owl:Class>
    


    <!-- http://purl.org/NET/atpir-cw#ProofDocument -->

    <owl:Class rdf:about="&atpir-fi;#ProofDocument">
        <rdfs:comment>Any kind of documents that can prove the legal arguments, facts, sustained in the complaint against the air carrier (in particular boarding passes, flight records as well as correspondence with the aircarrier).</rdfs:comment>
    </owl:Class>
    


    <!-- http://purl.org/NET/atpir-cw#SubmitingToNationalEnforcementBody -->

    <owl:Class rdf:about="&atpir-fi;#SubmitingToNationalEnforcementBody">
        <rdfs:subClassOf rdf:resource="&atpir-fi;#ActionStep"/>
        <rdfs:comment>Second step of the complaint workflow that consist in submiting the complaint to the National Enforcement Body.</rdfs:comment>
    </owl:Class>
    


    <!-- http://purl.org/NET/atpir-cw#TechnicalCrew -->

    <owl:Class rdf:about="&atpir-fi;#TechnicalCrew">
        <rdfs:subClassOf rdf:resource="&atpir-fi;#AirCarrier"/>
        <rdfs:comment>Technical crew include flight deck positions, which consists of those who fly the plane.</rdfs:comment>
    </owl:Class>
    


    <!-- http://purl.org/NET/atpir-cw#TicketReceipt -->

    <owl:Class rdf:about="&atpir-fi;#TicketReceipt">
        <rdfs:subClassOf rdf:resource="&atpir-fi;#ProofDocument"/>
        <rdfs:comment>A receipt is a written acknowledgment that a specified article or payment has been received.</rdfs:comment>
    </owl:Class>
    


    <!-- http://purl.org/NET/atpir-cw#TravelAgency -->

    <owl:Class rdf:about="&atpir-fi;#TravelAgency">
        <rdfs:subClassOf rdf:resource="&atpir-fi;#Party"/>
        <rdfs:comment>A travel agency is a private retailer or public service that provides travel and tourism related services to the public on behalf of suppliers such as airlines, car rentals, cruise lines, hotels, railways, and package tours.</rdfs:comment>
    </owl:Class>
    


    <!-- 
    ///////////////////////////////////////////////////////////////////////////////////////
    //
    // Individuals
    //
    ///////////////////////////////////////////////////////////////////////////////////////
     -->

    


    <!-- http://purl.org/NET/atpir-cw#EUComplaintForm -->

    <owl:NamedIndividual rdf:about="&atpir-fi;#EUComplaintForm">
        <rdf:type rdf:resource="&atpir-fi;#OnlineComplaining"/>
    </owl:NamedIndividual>
    


    <!-- http://purl.org/NET/atpir-cw#Email -->

    <owl:NamedIndividual rdf:about="&atpir-fi;#Email">
        <rdf:type rdf:resource="&atpir-fi;#OnlineComplaining"/>
    </owl:NamedIndividual>
    


    <!-- http://purl.org/NET/atpir-cw#Fax -->

    <owl:NamedIndividual rdf:about="&atpir-fi;#Fax">
        <rdf:type rdf:resource="&atpir-fi;#OnlineComplaining"/>
    </owl:NamedIndividual>
    


    <!-- http://purl.org/NET/atpir-cw#Webform -->

    <owl:NamedIndividual rdf:about="&atpir-fi;#Webform">
        <rdf:type rdf:resource="&atpir-fi;#OnlineComplaining"/>
    </owl:NamedIndividual>
</rdf:RDF>



<!-- Generated by the OWL API (version 3.5.1) http://owlapi.sourceforge.net -->

